@prefix : <https://docs.dynamicdashboard.ilabt.imec.be/ontologies/visualizations#> .
@prefix owl: <http://www.w3.org/2002/07/owl#> .
@prefix rdf: <http://www.w3.org/1999/02/22-rdf-syntax-ns#> .
@prefix xml: <http://www.w3.org/XML/1998/namespace> .
@prefix xsd: <http://www.w3.org/2001/XMLSchema#> .
@prefix rdfs: <http://www.w3.org/2000/01/rdf-schema#> .
@prefix dashb: <https://docs.dynamicdashboard.ilabt.imec.be/ontologies/dashboard#> .
@base <https://docs.dynamicdashboard.ilabt.imec.be/ontologies/visualizations#> .

: rdf:type owl:Ontology ;
  rdfs:label "The Dynamic Dashboard Visualizations Ontology" ;
  owl:imports <https://docs.dynamicdashboard.ilabt.imec.be/ontologies/dashboard#> ;
  <http://purl.org/dc/terms/creator> "Sander Vanden Hautte", "Pieter Moens", "Emile Deman" .

#################################################################
#    Annotation properties
#################################################################

###  http://www.w3.org/2004/02/skos/core#definition
<http://www.w3.org/2004/02/skos/core#definition> rdf:type owl:AnnotationProperty .


#################################################################
#    Classes
#################################################################

###  https://docs.dynamicdashboard.ilabt.imec.be/ontologies/dashboard#Visualization
dashb:Visualization rdf:type owl:Class ;
                    rdfs:label "Visualization"@en .


###  https://docs.dynamicdashboard.ilabt.imec.be/ontologies/visualizations#ColumnChart
:ColumnChart rdf:type owl:Class ;
             rdfs:subClassOf dashb:Visualization ;
             rdfs:label "Column chart"@en ;
             <http://www.w3.org/2004/02/skos/core#definition> "A visualization that displays one or more quantities with a column (vertical bar), next to each other if there are multiple."@en .


###  https://docs.dynamicdashboard.ilabt.imec.be/ontologies/visualizations#Gauge
:Gauge rdf:type owl:Class ;
       rdfs:subClassOf dashb:Visualization ;
       rdfs:label "Gauge"@en ;
       <http://www.w3.org/2004/02/skos/core#definition> "A visualization that displays any quantity on a round axis."@en .


###  https://docs.dynamicdashboard.ilabt.imec.be/ontologies/visualizations#HistoricalDataVisualization
:HistoricalDataVisualization rdf:type owl:Class ;
                             rdfs:subClassOf dashb:Visualization ;
                             rdfs:label "Historical data visualization"@en .


###  https://docs.dynamicdashboard.ilabt.imec.be/ontologies/visualizations#LineChart
:LineChart rdf:type owl:Class ;
           rdfs:subClassOf dashb:Visualization ;
           rdfs:label "Line chart"@en ;
           <http://www.w3.org/2004/02/skos/core#definition> "A visualization that displays any quantity, usually against time, on a orthogonal 2-axis plotting space."@en .


###  https://docs.dynamicdashboard.ilabt.imec.be/ontologies/visualizations#Map
:Map rdf:type owl:Class ;
     rdfs:subClassOf dashb:Visualization ;
     rdfs:label "Map"@en ;
     <http://www.w3.org/2004/02/skos/core#definition> "A visualization that displays locations, using their latitude and longitude."@en .


###  https://docs.dynamicdashboard.ilabt.imec.be/ontologies/visualizations#PieChart
:PieChart rdf:type owl:Class ;
          rdfs:subClassOf dashb:Visualization ;
          rdfs:label "Pie chart"@en ;
          <http://www.w3.org/2004/02/skos/core#definition> "A visualization that displays a pie, divided in slices corresponding with quantities that have been observed."@en .


###  https://docs.dynamicdashboard.ilabt.imec.be/ontologies/visualizations#RealtimeDataVisualization
:RealtimeDataVisualization rdf:type owl:Class ;
                           rdfs:subClassOf dashb:Visualization ;
                           rdfs:label "Real-time data visualization"@en .


###  https://docs.dynamicdashboard.ilabt.imec.be/ontologies/visualizations#ScatterPlot
:ScatterPlot rdf:type owl:Class ;
             rdfs:subClassOf dashb:Visualization ;
             rdfs:label "Scatter plot"@en ;
             <http://www.w3.org/2004/02/skos/core#definition> "A visualization that displays all observed data points of a certain quantity."@en .


###  https://docs.dynamicdashboard.ilabt.imec.be/ontologies/visualizations#Thermometer
:Thermometer rdf:type owl:Class ;
             rdfs:subClassOf dashb:Visualization ;
             rdfs:label "Thermometer"@en ;
             <http://www.w3.org/2004/02/skos/core#definition> "A visualization that displays temperatures."@en .


###  https://docs.dynamicdashboard.ilabt.imec.be/ontologies/visualizations#WindRose
:WindRose rdf:type owl:Class ;
          rdfs:subClassOf dashb:Visualization ;
          rdfs:label "Wind rose"@en ;
          <http://www.w3.org/2004/02/skos/core#definition> "A visualization that displays wind directions, sometimes combined with wind speeds."@en .


###  Generated by the OWL API (version 4.5.13) https://github.com/owlcs/owlapi
